fixed up polydemos

tests/PolyDemos.v
@@ -30,7 +30,7 @@ Notation list_A := (TEApp
 Notation nat_ty := (TEVar (TEVNamed sort_nat)).
 
 Inductive demo_funs : 
-  forall ctx, list (ty_expr demo_sorts ctx 0) -> ty_expr demo_sorts ctx 0 -> Type := 
+  forall ctx, list (@ty_expr demo_sorts ctx 0) -> @ty_expr demo_sorts ctx 0 -> Type := 
 | demo_app : demo_funs 1 [list_A; list_A] list_A (* forall A, list A -> list A -> list A*)
 | demo_len : demo_funs 1 [list_A] nat_ty (* forall A, list A -> nat *)
 | demo_add : demo_funs 0 [nat_ty; nat_ty] nat_ty (* nat -> nat -> nat *)
@@ -38,9 +38,9 @@ Inductive demo_funs :
 .
 
 Inductive demo_rels : 
-  forall ctx, list (ty_expr demo_sorts ctx 0) -> Type := .
+  forall ctx, list (@ty_expr demo_sorts ctx 0) -> Type := .
 
-Definition demo_sig : signature demo_sorts := {|
+Definition demo_sig : @signature demo_sorts := {|
   sig_funs := demo_funs;
   sig_rels := demo_rels;
 |}.
@@ -52,24 +52,21 @@ Definition interp_demo_sorts : forall n, demo_sorts n -> arity_ftor n := fun n s
   end.
 
 Equations 
-  interp_demo_funs t_ctx ctx args ret (fn: demo_funs t_ctx args ret) tv (hargs: HList.t (interp_te demo_sorts interp_demo_sorts t_ctx ctx tv 0) args) : 
-  interp_te demo_sorts interp_demo_sorts t_ctx ctx tv 0 ret := {
+  interp_demo_funs t_ctx ctx args ret (fn: demo_funs t_ctx args ret) tv (hargs: HList.t (interp_te (interp_sorts := interp_demo_sorts) t_ctx ctx tv 0) args) : 
+  interp_te (interp_sorts := interp_demo_sorts) t_ctx ctx tv 0 ret := {
   interp_demo_funs _ _ _ _ demo_app _ (l ::: r ::: _) := List.app l r; 
   interp_demo_funs _ _ _ _ demo_len _ (x ::: _) := List.length x; 
   interp_demo_funs _ _ _ _ demo_add _ (l ::: r ::: _) := l + r; 
   interp_demo_funs _ _ _ _ demo_zero _ _ := 0; 
 }.
 
-Definition interp_demo_rels t_ctx ctx args (fn: demo_rels t_ctx args) tv (hargs: HList.t (interp_te demo_sorts interp_demo_sorts t_ctx ctx tv 0) args) : Prop := 
+Definition interp_demo_rels t_ctx ctx args (fn: demo_rels t_ctx args) tv (hargs: HList.t (interp_te (interp_sorts := interp_demo_sorts) t_ctx ctx tv 0) args) : Prop := 
   match fn with end.
 
-Program Definition demo_model : interp_sig demo_sorts interp_demo_sorts demo_sig := {| 
+Program Definition demo_model : interp_sig demo_sig := {| 
   interp_funs := interp_demo_funs;
   interp_rels := interp_demo_rels;
 |}.
-
-
-
 
 Notation t_xs := (TVar (VThere VHere)).
 Notation t_ys := (TVar VHere).
@@ -80,16 +77,16 @@ Notation t_add args := (TFun (sig := demo_sig) demo_add TVEmp args).
 Notation t_zero := (TFun (sig := demo_sig) demo_zero TVEmp hnil).
 
 Program Definition app_len_pf_syntax: 
-  poly_fm demo_sorts demo_sig 0 :=  PForall (PFm (
+  poly_fm (sig := demo_sig) 0 :=  PForall (PFm (
     FForall list_A (FForall list_A (
       FEq 
         (t_len _ ((t_app _ (t_xs ::: t_ys ::: hnil)) ::: hnil))
-        (t_add ((t_len (TVSnoc _ loc_A _ TVEmp) (t_xs ::: hnil)) ::: (t_len _ (t_ys ::: hnil)) ::: hnil))
+        (t_add ((t_len (TVSnoc TVEmp loc_A) (t_xs ::: hnil)) ::: (t_len _ (t_ys ::: hnil)) ::: hnil))
     ))
   )).
 
 Example app_len_pf: 
-  interp_pfm demo_sorts interp_demo_sorts demo_sig demo_model 0 SLNil TVEmp app_len_pf_syntax.
+  interp_pfm (model := demo_model) 0 SLNil TVEmp app_len_pf_syntax.
 Proof.
   (* this short proof works as well: *)
   (* 
@@ -99,7 +96,7 @@ Proof.
   *)
   unfold app_len_pf_syntax.
   autorewrite with interp_pfm.
-  unfold interp_pfm_obligations_obligation_1, interp_pfm_obligations_obligation_2.
+  unfold PolyFirstOrder.interp_pfm_obligations_obligation_1, PolyFirstOrder.interp_pfm_obligations_obligation_2.
   intros.
   autorewrite with interp_pfm.
   autorewrite with interp_fm.
@@ -108,17 +105,17 @@ Proof.
   autorewrite with interp_fm.
   intros.
   vm_compute in x0.
-  set (t := apply_ty_args _ _ _ _ _ _ _).
+  set (t := apply_ty_args _ _ _ _ _ _).
   vm_compute in t.
   subst t.
   autorewrite with interp_fm.
-  unfold interp_fm_obligations_obligation_1, interp_fm_obligations_obligation_2, interp_fm_obligations_obligation_3, interp_fm_obligations_obligation_4.
-  set (t := apply_ty_args _ _ _ _ _ _ _);
+  unfold PolyFirstOrder.interp_fm_obligations_obligation_1, PolyFirstOrder.interp_fm_obligations_obligation_2, PolyFirstOrder.interp_fm_obligations_obligation_3, PolyFirstOrder.interp_fm_obligations_obligation_4.
+  set (t := apply_ty_args _ _ _ _ _ _);
   vm_compute in t;
   subst t.
 
-  set (l := interp_tm _ _ _ _ _ _ _ _ _ _ _).
-  set (r := interp_tm _ _ _ _ _ _ _ _ _ _ _).
+  set (l := interp_tm _ _ _ _ _ _ _).
+  set (r := interp_tm _ _ _ _ _ _ _).
   vm_compute in l.
   vm_compute in r.
   eapply List.app_length.
@@ -137,21 +134,21 @@ Inductive generic_sorts: nat -> Type :=
 | generic_inner: forall n, generic_inner_sorts n -> generic_sorts n.
 
 Notation loc_A := (TEVar (TEVAnon TCVHere)).
-Notation loc_B := (TEVar (TEVAnon (TCVThere _ TCVHere))).
+Notation loc_B := (TEVar (TEVAnon (TCVThere TCVHere))).
 
 Notation arrow_A_B := (TEApp (TEApp (TEVar (TEVNamed generic_arrow)) loc_A) loc_B).
 
 Import ListNotations.
 
 Inductive generic_funs:
-  forall ctx, list (ty_expr generic_sorts ctx 0) -> ty_expr generic_sorts ctx 0 -> Type :=
+  forall ctx, list (ty_expr (sig_sorts := generic_sorts) ctx 0) -> ty_expr (sig_sorts := generic_sorts) ctx 0 -> Type :=
 | generic_eval : generic_funs 2 [arrow_A_B; loc_A] loc_B (* forall A B, arrow A B -> A -> B*)
 .
 
 Inductive generic_rels:
-  forall ctx, list (ty_expr generic_sorts ctx 0) -> Type := .
+  forall ctx, list (ty_expr (sig_sorts := generic_sorts) ctx 0) -> Type := .
 
-Definition generic_sig: signature generic_sorts := {|
+Definition generic_sig: @signature generic_sorts := {|
   sig_funs := generic_funs;
   sig_rels := generic_rels;
 |}.
@@ -165,15 +162,15 @@ Equations interp_generic_sorts n (sort: generic_sorts n) : arity_ftor n := {
 
 Equations
   interp_generic_funs t_ctx ctx args ret (fn: generic_funs t_ctx args ret)
-    tv (hargs: HList.t (interp_te generic_sorts interp_generic_sorts t_ctx ctx tv 0) args) :
-  interp_te generic_sorts interp_generic_sorts t_ctx ctx tv 0 ret := {
+    tv (hargs: HList.t (interp_te (interp_sorts := interp_generic_sorts) t_ctx ctx tv 0) args) :
+  interp_te (interp_sorts := interp_generic_sorts) t_ctx ctx tv 0 ret := {
   interp_generic_funs _ _ _ _ generic_eval _ (f ::: arg ::: _) := f arg;
 }.
 
-Definition interp_generic_rels t_ctx ctx args (rel: generic_rels t_ctx args) tv (hargs: HList.t (interp_te generic_sorts interp_generic_sorts t_ctx ctx tv 0) args) : Prop :=
+Definition interp_generic_rels t_ctx ctx args (rel: generic_rels t_ctx args) tv (hargs: HList.t (interp_te (interp_sorts := interp_generic_sorts) t_ctx ctx tv 0) args) : Prop :=
   match rel with end.
 
-Program Definition generic_model : interp_sig generic_sorts interp_generic_sorts generic_sig := {|
+Program Definition generic_model : interp_sig generic_sig := {|
   interp_funs := interp_generic_funs;
   interp_rels := interp_generic_rels;
 |}.
@@ -186,6 +183,8 @@ Inductive generic_inner_sorts : nat -> Type :=
 | inner_sort_list : generic_inner_sorts 1
 | inner_sort_nat : generic_inner_sorts 0.
 
+Check TVSnoc.
+
 Notation te_arrow A B := (TEApp (TEApp (TEVar (TEVNamed (generic_arrow generic_inner_sorts))) A) B).
 Notation loc_A := (TEVar (TEVAnon TCVHere)).
 Notation list_A := (TEApp (TEVar (TEVNamed (generic_inner _ _ inner_sort_list))) loc_A).
@@ -195,23 +194,23 @@ Notation app_A := (te_arrow list_A (te_arrow list_A list_A)).
 Notation cons_A := (te_arrow loc_A (te_arrow list_A list_A)).
 Notation add' := (te_arrow nat' (te_arrow nat' nat')).
 Notation t_eval ty_args args := (TFun (sig := generic_sig generic_inner_sorts) (generic_eval _) ty_args args).
-Notation t_len_A arg := (t_eval (TVSnoc _ list_A _ (TVSnoc _ nat' _ TVEmp))
+Notation t_len_A arg := (t_eval (TVSnoc (TVSnoc TVEmp nat') list_A)
                                  (TVar (VThere (VThere (VThere (VThere (VThere VHere))))) ::: arg ::: hnil)).
-Notation t_app_A x y := (t_eval (TVSnoc _ list_A _ (TVSnoc _ list_A _ TVEmp))
-                              (t_eval (TVSnoc _ list_A _ (TVSnoc _ (te_arrow list_A list_A) _ TVEmp))
+Notation t_app_A x y := (t_eval (TVSnoc (TVSnoc TVEmp list_A ) list_A )
+                              (t_eval (TVSnoc (TVSnoc TVEmp (te_arrow list_A list_A)) list_A)
                               (TVar (VThere (VThere (VThere (VThere (VThere VHere))))) ::: x ::: hnil) ::: y ::: hnil)).
-Notation t_app_A' x y := (t_eval (TVSnoc _ list_A _ (TVSnoc _ list_A _ TVEmp))
-                              (t_eval (TVSnoc _ list_A _ (TVSnoc _ (te_arrow list_A list_A) _ TVEmp))
+Notation t_app_A' x y := (t_eval (TVSnoc (TVSnoc TVEmp list_A) list_A)
+                              (t_eval (TVSnoc  (TVSnoc TVEmp (te_arrow list_A list_A)) list_A)
                               (TVar (VThere (VThere (VThere (VThere VHere)))) ::: x ::: hnil) ::: y ::: hnil)).
-Notation t_cons_A a x := (t_eval (TVSnoc _ list_A _ (TVSnoc _ list_A _ TVEmp))
-                              (t_eval (TVSnoc _ loc_A _ (TVSnoc _ (te_arrow list_A list_A) _ TVEmp))
+Notation t_cons_A a x := (t_eval (TVSnoc (TVSnoc TVEmp list_A) list_A)
+                              (t_eval (TVSnoc (TVSnoc TVEmp (te_arrow list_A list_A)) loc_A)
                               (TVar (VThere (VThere (VThere (VThere VHere)))) ::: a ::: hnil) ::: x ::: hnil)).
-Notation t_add' x y := (t_eval (TVSnoc _ nat' _ (TVSnoc _ nat' _ TVEmp))
-                              (t_eval (TVSnoc _ nat' _ (TVSnoc _ (te_arrow nat' nat') _ TVEmp))
+Notation t_add' x y := (t_eval (TVSnoc (TVSnoc TVEmp nat' ) nat')
+                              (t_eval (TVSnoc (TVSnoc TVEmp (te_arrow nat' nat')) nat')
                               (TVar (VThere (VThere VHere)) ::: x ::: hnil) ::: y ::: hnil)).
 
 Check FForall add' (
-    FImpl _ _ _ _
+    FImpl 
         (
         FForall loc_A (
         FForall list_A (
@@ -228,14 +227,16 @@ Check FForall add' (
         )))
     ).
 
+Check poly_fm.
+
 Definition generic_test:
-  poly_fm (generic_sorts generic_inner_sorts) (generic_sig generic_inner_sorts) 0 :=
+  poly_fm 0 :=
   PForall (PFm (
     FForall len_A (
     FForall app_A (
     FForall cons_A (
     FForall add' (
-    FImpl _ _ _ _
+    FImpl
         (
         FForall loc_A (
     FForall list_A (
@@ -260,7 +261,8 @@ Definition interp_generic_sorts_inner : forall n, generic_inner_sorts n -> arity
   end.
 
 Example app_len_generic:
-    interp_pfm (generic_sorts generic_inner_sorts) (interp_generic_sorts generic_inner_sorts interp_generic_sorts_inner) (generic_sig generic_inner_sorts) (generic_model generic_inner_sorts interp_generic_sorts_inner) 0 SLNil TVEmp generic_test.
+    interp_pfm (model := generic_model generic_inner_sorts interp_generic_sorts_inner) 
+      0 SLNil TVEmp generic_test.
 Proof.
   vm_compute.
 Abort.
@@ -278,28 +280,28 @@ Inductive parametrized_sorts: nat -> Type :=
 | parametrized_inner: forall n, parametrized_inner_sorts n -> parametrized_sorts n.
 
 Definition parametrized_manifest :=
-    list {ctx & list (ty_expr parametrized_sorts ctx 0) *
-                ty_expr parametrized_sorts ctx 0}.
+    list {ctx & list (@ty_expr parametrized_sorts ctx 0) *
+                @ty_expr parametrized_sorts ctx 0}.
 
 Inductive parametrized_funs_open:
     parametrized_manifest ->
     forall ctx,
-    list (ty_expr parametrized_sorts ctx 0) ->
-    ty_expr parametrized_sorts ctx 0 ->
+    list (@ty_expr parametrized_sorts ctx 0) ->
+    @ty_expr parametrized_sorts ctx 0 ->
     Type
 :=
 | PFunHere:
     forall ctx
            tail
-           (args: list (ty_expr parametrized_sorts ctx 0))
-           (ret: ty_expr parametrized_sorts ctx 0),
+           (args: list (@ty_expr parametrized_sorts ctx 0))
+           (ret: @ty_expr parametrized_sorts ctx 0),
         parametrized_funs_open (existT _ ctx (args, ret) :: tail) ctx args ret
 | PFunThere:
     forall ctx
            head
            tail
-           (args: list (ty_expr parametrized_sorts ctx 0))
-           (ret: ty_expr parametrized_sorts ctx 0),
+           (args: list (@ty_expr parametrized_sorts ctx 0))
+           (ret: @ty_expr parametrized_sorts ctx 0),
         parametrized_funs_open tail ctx args ret ->
         parametrized_funs_open (head :: tail) ctx args ret
 .
@@ -309,9 +311,9 @@ Variable parametrized_inner_funcs: parametrized_manifest.
 Definition parametrized_funs := parametrized_funs_open parametrized_inner_funcs.
 
 Inductive parametrized_rels:
-  forall ctx, list (ty_expr parametrized_sorts ctx 0) -> Type := .
+  forall ctx, list (@ty_expr parametrized_sorts ctx 0) -> Type := .
 
-Definition parametrized_sig: signature parametrized_sorts := {|
+Definition parametrized_sig: @signature parametrized_sorts := {|
   sig_funs := parametrized_funs;
   sig_rels := parametrized_rels;
 |}.
@@ -338,16 +340,16 @@ Inductive abstract_sorts: nat -> Type :=
 
 Variable inner_funs:
   forall ctx,
-    list (ty_expr inner_sorts ctx 0) ->
-    ty_expr inner_sorts ctx 0 ->
+    list (@ty_expr inner_sorts ctx 0) ->
+    @ty_expr inner_sorts ctx 0 ->
     Type
 .
 
 Equations abstract_ty_expr_var
   {n ctx}
-  (var: ty_expr_var inner_sorts ctx n)
+  (var: @ty_expr_var inner_sorts ctx n)
 :
-  ty_expr_var abstract_sorts ctx n
+  @ty_expr_var abstract_sorts ctx n
 := {
   abstract_ty_expr_var (TEVAnon var) :=
     TEVAnon var;
@@ -357,9 +359,9 @@ Equations abstract_ty_expr_var
 
 Equations abstract_ty_expr
   {n ctx}
-  (var: ty_expr inner_sorts ctx n)
+  (var: @ty_expr inner_sorts ctx n)
 :
-  ty_expr abstract_sorts ctx n
+  @ty_expr abstract_sorts ctx n
 := {
   abstract_ty_expr (TEVar var) :=
     TEVar (abstract_ty_expr_var var);
@@ -370,8 +372,8 @@ Equations abstract_ty_expr
 
 Inductive abstract_funs:
   forall ctx,
-    list (ty_expr abstract_sorts ctx 0) ->
-    ty_expr abstract_sorts ctx 0 ->
+    list (ty_expr ctx 0) ->
+    @ty_expr abstract_sorts ctx 0 ->
     Type
 :=
 | abstract_inner_fun:
@@ -383,13 +385,13 @@ Inductive abstract_funs:
 
 Variable inner_rels:
   forall ctx,
-    list (ty_expr inner_sorts ctx 0) ->
+    list (@ty_expr inner_sorts ctx 0) ->
     Type
 .
 
 Inductive abstract_rels:
   forall ctx,
-    list (ty_expr abstract_sorts ctx 0) ->
+    list (ty_expr ctx 0) ->
     Type
 :=
 | abstract_inner_rel:
@@ -398,7 +400,7 @@ Inductive abstract_rels:
       abstract_rels ctx (map abstract_ty_expr args)
 .
 
-Definition abstract_sig: signature abstract_sorts := {|
+Definition abstract_sig: @signature abstract_sorts := {|
   sig_funs := abstract_funs;
   sig_rels := abstract_rels;
 |}.
@@ -413,19 +415,19 @@ Equations interp_abstract_sorts n (sort: abstract_sorts n) : arity_ftor n := {
 
 Variable interp_inner_funs:
   forall t_ctx ctx args ret (fn: inner_funs t_ctx args ret) tv
-    (hargs: HList.t (interp_te inner_sorts interp_inner_sorts t_ctx ctx tv 0) args),
-    interp_te inner_sorts interp_inner_sorts t_ctx ctx tv 0 ret
+    (hargs: HList.t (@interp_te _ interp_inner_sorts t_ctx ctx tv 0) args),
+    @interp_te _ interp_inner_sorts t_ctx ctx tv 0 ret
 .
 
 Equations concretize_interp_te_var 
   t_ctx ctx tv te_var 
-  (val: interp_te_var abstract_sorts interp_abstract_sorts ctx t_ctx tv 0 (abstract_ty_expr_var te_var)) 
-: interp_te_var inner_sorts interp_inner_sorts ctx t_ctx tv 0 te_var := {
+  (val: interp_te_var (interp_sorts := interp_abstract_sorts) ctx t_ctx tv 0 (abstract_ty_expr_var te_var)) 
+: interp_te_var (interp_sorts := interp_inner_sorts) ctx t_ctx tv 0 te_var := {
   concretize_interp_te_var _ _ _ (TEVAnon _) val := val;
   concretize_interp_te_var _ _ _ (TEVNamed _) val := val;
 }.
 
-Definition concretize_interp_te t_ctx ctx tv n ty_expr: interp_te abstract_sorts interp_abstract_sorts t_ctx ctx tv n (abstract_ty_expr ty_expr) = interp_te inner_sorts interp_inner_sorts t_ctx ctx tv n ty_expr.
+Definition concretize_interp_te t_ctx ctx tv n ty_expr: interp_te (interp_sorts := interp_abstract_sorts) t_ctx ctx tv n (abstract_ty_expr ty_expr) = interp_te (interp_sorts := interp_inner_sorts) t_ctx ctx tv n ty_expr.
 Proof.
   dependent induction ty_expr; autorewrite with abstract_ty_expr.
   - autorewrite with abstract_ty_expr.
@@ -434,7 +436,7 @@ Proof.
     now rewrite IHty_expr1, IHty_expr2.
 Defined.
 
-Definition concretize_interp_te' t_ctx ctx tv ty_expr: interp_te abstract_sorts interp_abstract_sorts t_ctx ctx tv 0 (abstract_ty_expr ty_expr) -> interp_te inner_sorts interp_inner_sorts t_ctx ctx tv 0 ty_expr.
+Definition concretize_interp_te' t_ctx ctx tv ty_expr: interp_te (interp_sorts := interp_abstract_sorts) t_ctx ctx tv 0 (abstract_ty_expr ty_expr) -> interp_te (interp_sorts := interp_inner_sorts) t_ctx ctx tv 0 ty_expr.
 Proof.
   intro.
   now rewrite concretize_interp_te in X.
@@ -451,8 +453,8 @@ Equations
   interp_abstract_funs 
     t_ctx ctx args ret 
     (fn: abstract_funs t_ctx args ret) tv 
-    (hargs: HList.t (interp_te abstract_sorts interp_abstract_sorts t_ctx ctx tv 0) args) 
-: interp_te abstract_sorts interp_abstract_sorts t_ctx ctx tv 0 ret := {
+    (hargs: HList.t (interp_te (interp_sorts := interp_abstract_sorts) t_ctx ctx tv 0) args) 
+: interp_te (interp_sorts := interp_abstract_sorts) t_ctx ctx tv 0 ret := {
   interp_abstract_funs _ _ _ _ (abstract_inner_fun _ _ _ inner_fun) _ args := 
     let swapped := HList.map_swap _ _ args in 
       _;
@@ -470,7 +472,7 @@ Defined.
 
 Variable interp_inner_rels:
   forall t_ctx ctx args (fn: inner_rels t_ctx args) tv
-    (hargs: HList.t (interp_te inner_sorts interp_inner_sorts t_ctx ctx tv 0) args),
+    (hargs: HList.t (interp_te (interp_sorts := interp_inner_sorts) t_ctx ctx tv 0) args),
     Prop
 .
 
@@ -478,7 +480,7 @@ Equations
   interp_abstract_rels 
     t_ctx ctx args 
     (fn: abstract_rels t_ctx args) tv 
-    (hargs: HList.t (interp_te abstract_sorts interp_abstract_sorts t_ctx ctx tv 0) args) 
+    (hargs: HList.t (interp_te (interp_sorts := interp_abstract_sorts) t_ctx ctx tv 0) args) 
 : Prop := {
   interp_abstract_rels _ _ _ (abstract_inner_rel _ _ inner_rel) _ args := 
     let swapped := HList.map_swap _ _ args in 
@@ -495,27 +497,29 @@ exact X.
 Defined.
 
 
-Program Definition abstract_model : interp_sig abstract_sorts interp_abstract_sorts abstract_sig := {|
+Program Definition abstract_model : interp_sig abstract_sig := {|
   interp_funs := interp_abstract_funs;
   interp_rels := interp_abstract_rels;
 |}.
 
-Definition inner_sig : signature inner_sorts := {| 
+Definition inner_sig : @signature inner_sorts := {| 
   sig_funs := inner_funs;
   sig_rels := inner_rels;
 |}.
 
-Fixpoint get_poly_context {ctx} (pfm: poly_fm inner_sorts inner_sig ctx) : ty_ctx :=
+Fixpoint get_poly_context {ctx} (pfm: poly_fm (sig := inner_sig) ctx) : ty_ctx :=
   match pfm with 
   | PFm _ => ctx
   | PForall inner => 
     get_poly_context inner
   end.
 
-Fixpoint get_poly_fm {ctx} (pfm: poly_fm inner_sorts inner_sig ctx) : fm inner_sorts inner_sig (get_poly_context pfm) SLNil := 
+Fixpoint get_poly_fm {ctx} (pfm: poly_fm (sig := inner_sig) ctx) : fm (sig := inner_sig) (t_ctx := get_poly_context pfm) SLNil := 
   match pfm with 
   | PFm f => f
   | PForall inner => get_poly_fm inner
   end.
 
 (* TODO: walk the term and rewrite function and relation symbols; prove the two are bi-satisfactory *)
+
+End ConstantTypesAbstractedTheory.
